isolate Steel.C.Array-specific parts

src/lowparse/steel_c_array/LowParse.Steel.ArrayPtr.fst
@@ -1,4 +1,5 @@
 module LowParse.Steel.ArrayPtr
+friend LowParse.Steel.StdInt
 
 module A = Steel.C.Array
 module R = Steel.Reference
@@ -565,24 +566,3 @@ let free #base #a r =
     (A.varray ar);
   A.free ar;
   R.ghost_free (fst0 tmp)
-
-let array_of x = x
-
-let enter #_ #base #t0 ar =
-    let tmp : R.ghost_ref (array' (fst0 ar)) = R.ghost_alloc ar in
-    array_null_to_unique ar;
-    let res : t base t0 = (fst0 ar, Ghost.hide (Some ({ from = fst0 ar; to = tmp; }))) in
-    change_equal_slprop
-      (R.ghost_vptr tmp)
-      (R.ghost_vptr (Some?.v (snd0 res)).to);
-    intro_varrayptr res ar ();
-    return res
-
-let exit #_ #base #a r =
-  let tmp = elim_varrayptr r in
-  let ar : A.array base a = (fst0 r, snd0 (snd0 tmp)) in
-  change_equal_slprop
-    (A.varray (snd0 tmp))
-    (A.varray ar);
-  R.ghost_free (fst0 tmp);
-  return ar
