src/lowparse/LowParse.Steel.StdInt.fsti
@@ -1,0 +1,60 @@
+// TODO: replace with Steel.C.StdInt once FStar#2349 is merged
+module LowParse.Steel.StdInt
+
+open FStar.Mul
+
+module U32 = FStar.UInt32
+module I32 = FStar.Int32
+
+inline_for_extraction noextract // TODO: replace with primitive extraction
+val size_t : eqtype
+
+val size_precond (x: nat) : Tot prop
+
+noextract
+val size_v (x: size_t) : Pure nat // should be Ghost, but need Pure to implement alloc
+  (requires True)
+  (ensures (fun y -> size_precond y))
+
+val size_v_inj (x1 x2: size_t) : Lemma
+  (size_v x1 == size_v x2 ==> x1 == x2)
+  [SMTPat (size_v x1); SMTPat (size_v x2)]
+
+inline_for_extraction noextract
+val mk_size_t (x: U32.t) : Pure size_t
+  (requires True)
+  (ensures (fun y -> size_v y == U32.v x))
+
+noextract
+val int_to_size_t (x: nat) : Pure size_t // should be Ghost, but need Pure to implement array views
+  (requires (size_precond x))
+  (ensures (fun y -> size_v y == x))
+
+val size_precond_le (x y: nat) : Lemma
+  (requires (x <= y /\ size_precond y))
+  (ensures (size_precond x))
+  [SMTPat (size_precond x); SMTPat (size_precond y)]
+
+val size_add (x y: size_t) : Pure size_t
+  (requires (size_precond (size_v x + size_v y)))
+  (ensures (fun z -> size_v z == size_v x + size_v y))
+
+val size_sub (x y: size_t) : Pure size_t
+  (requires (size_v x >= size_v y))
+  (ensures (fun z -> size_v z == size_v x - size_v y))
+
+val size_mul (x y: size_t) : Pure size_t
+  (requires (size_precond (size_v x * size_v y)))
+  (ensures (fun z -> size_v z == size_v x * size_v y))
+
+val size_div (x y: size_t) : Pure size_t
+  (requires (size_v y > 0))
+  (ensures (fun z -> size_v z == size_v x / size_v y))
+
+val size_le (x y: size_t) : Pure bool
+  (requires True)
+  (ensures (fun z -> z == (size_v x <= size_v y)))
+
+let zero_size : (zero_size: size_t { size_v zero_size == 0 }) = mk_size_t 0ul
+
+let one_size : (zero_size: size_t { size_v zero_size == 1 }) = mk_size_t 1ul
