src/lowparse/steel_c_array/LowParse.Steel.ArrayPtr.Make.fst
@@ -1,0 +1,25 @@
+module LowParse.Steel.ArrayPtr.Make
+friend LowParse.Steel.ArrayPtr
+
+module R = Steel.Reference
+
+let array_of x = x
+
+let enter #_ #base #t0 ar =
+    let tmp : R.ghost_ref (array' (fst0 ar)) = R.ghost_alloc ar in
+    array_null_to_unique ar;
+    let res : t base t0 = (fst0 ar, Ghost.hide (Some ({ from = fst0 ar; to = tmp; }))) in
+    change_equal_slprop
+      (R.ghost_vptr tmp)
+      (R.ghost_vptr (Some?.v (snd0 res)).to);
+    intro_varrayptr res ar ();
+    return res
+
+let exit #_ #base #a r =
+  let tmp = elim_varrayptr r in
+  let ar : A.array base a = (fst0 r, snd0 (snd0 tmp)) in
+  change_equal_slprop
+    (A.varray (snd0 tmp))
+    (A.varray ar);
+  R.ghost_free (fst0 tmp);
+  return ar
