src/lowparse/steel_c_array/LowParse.Steel.ArrayPtr.Make.fsti
@@ -1,0 +1,59 @@
+module LowParse.Steel.ArrayPtr.Make
+include LowParse.Steel.ArrayPtr
+
+open Steel.Memory
+open Steel.Effect
+open Steel.FractionalPermission
+open Steel.Effect.Atomic
+module SZ = LowParse.Steel.StdInt
+
+(* Entering and exiting the abstraction *)
+module A = Steel.C.Array
+
+val array_of
+  (#base #t: Type0)
+  (x: array base t)
+: Ghost (A.array base t)
+  (requires True)
+  (ensures (fun y -> A.length y == length x))
+
+inline_for_extraction
+val enter
+  (#opened: _)
+  (#base: Type)
+  (#a: Type)
+  (x: A.array base a)
+//  (p: perm)
+: SteelAtomicBase (t base a) false opened Unobservable
+    (A.varray x) // (A.varrayp x p)
+    (fun res -> varrayptr res)
+    (fun _ ->
+      True
+//      let p = A.g_get_pointer x in
+//      (P.g_is_null p == false ==> P.size_v (P.base_array_len (P.base p)) < 4294967296) // TODO: remove and use size_t instead
+    )
+    (fun h res h' ->
+      let s = h' (varrayptr res) in
+      array_of s.array == x /\
+//      s.perm == p /\
+      s.contents == h (A.varray x) // (A.varrayp x p)
+    )
+
+inline_for_extraction
+val exit
+  (#opened: _)
+  (#base: Type)
+  (#a: Type)
+  (x: t base a)
+: SteelAtomicBase (A.array base a) (* & perm *) false opened Unobservable
+    (varrayptr x)
+    (fun res -> A.varray res) // A.varrayp (fst res) (snd res))
+    (fun _ -> True)
+    (fun h res h' ->
+      let s = h (varrayptr x) in
+      res == array_of s.array /\
+      h' (A.varray res) == s.contents
+//      fst res == s.array /\
+//      snd res == s.perm /\
+//      h' (A.varrayp (fst res) (snd res)) == s.contents
+    )
