src/lowparse/steel_c_array/LowParse.Steel.StdInt.fst
@@ -1,0 +1,16 @@
+module LowParse.Steel.StdInt
+
+module SZ = Steel.C.StdInt.Base
+
+let size_t = SZ.size_t
+let size_precond = SZ.size_precond
+let size_v = SZ.size_v
+let size_v_inj = SZ.size_v_inj
+let mk_size_t = SZ.mk_size_t
+let int_to_size_t = SZ.int_to_size_t
+let size_precond_le = SZ.size_precond_le
+let size_add = SZ.size_add
+let size_sub = SZ.size_sub
+let size_mul = SZ.size_mul
+let size_div = SZ.size_div
+let size_le = SZ.size_le
